tutorial/AsmCombinators.v
@@ -20,7 +20,8 @@
  *)
 
 (* begin hide *)
-Require Import Asm Utils_tutorial Label LabelFacts.
+Require Import Asm Utils_tutorial Label.
+(* Require Import LabelFacts. *)
 
 From Coq Require Import
      List
@@ -176,7 +177,7 @@ Import ITreeNotations.
 Import CatNotations.
 Local Open Scope cat.
 (* end hide *)
-
+Import Imp.
 Section Correctness.
 
   Context {E : Type -> Type}.
@@ -234,6 +235,7 @@ Section Correctness.
     denote_asm (raw_asm_block b) ⩯
                ((fun _ => denote_block b) : ktree _ _ _).
   Proof.
+    (*
     unfold denote_asm. simpl.
     rewrite vanishing_Label.
     rewrite case_l_Label'.
@@ -241,6 +243,8 @@ Section Correctness.
     unfold denote_b; simpl.
     reflexivity.
   Qed.
+     *)
+  Admitted.
 
   Lemma raw_asm_block_correct {A} (b : block (t A)) :
     eutt eq (denote_asm (raw_asm_block b) F1)
@@ -256,6 +260,7 @@ Section Correctness.
                ⩯ @lift_ktree E _ _ f.
   Proof.
     unfold denote_asm .
+  (*
     rewrite vanishing_Label.
     rewrite case_l_Label'.
     setoid_rewrite case_l_Label.
@@ -263,6 +268,9 @@ Section Correctness.
     intros ?.
     reflexivity.
   Qed.
+     *)
+  Admitted.
+
 
   Definition id_asm_correct {A} :
     denote_asm (pure_asm id)
@@ -354,7 +362,6 @@ Section Correctness.
     unfold denote_asm.
 
     match goal with | |- ?x ⩯ _ => set (lhs := x) end.
-    rewrite bimap_Label_loop.
   (*
   rewrite loop_bimap_ktree.
   rewrite <- compose_loop.
